isabelle/Core/TimeRange.thy
@@ -1,0 +1,368 @@
+theory TimeRange
+imports Semantics PositiveAccounts QuiescentResult MoneyPreservation Timeout TransactionBound
+begin
+
+fun isCompatible :: "POSIXTime \<times> POSIXTime \<Rightarrow> POSIXTime option \<times> POSIXTime option \<Rightarrow> bool" where
+"isCompatible (min1, max1) (None, None) = True" |
+"isCompatible (_, max1) (None, Some max2) = (max1 \<le> max2)" |
+"isCompatible (min1, _) (Some min2, None) = (min1 \<ge> min2)" |
+"isCompatible (min1, max1) (Some min2, Some max2) = (min1 \<ge> min2 \<and> max1 \<le> max2)"
+
+theorem isCompatibleIdempotentToCombineInterval :
+  "isCompatible (min1, max1) (min2, max2) =
+     (combineIntervals (Some min1, Some max1) (min2, max2) = (Some min1, Some max1))"
+  apply (cases min2)
+  apply (cases max2)
+    apply simp
+  subgoal for a
+    by auto[1]
+    apply (cases max2)
+    subgoal for a
+      by auto
+    subgoal for a b
+      by auto
+    done
+
+lemma compatibleIdempotency1 :
+  "isCompatible (x, y) (combineIntervals b c) \<Longrightarrow> isCompatible (x, y) b"
+  apply (cases b)
+  apply (cases c)
+  subgoal for b1 b2 c1 c2
+    apply (simp only:combineIntervals.simps)
+    apply (cases b1)
+    apply (cases c1)
+    apply (smt (verit, best) Semantics.maxOpt.simps(1) Semantics.minOpt.elims TimeRange.isCompatible.simps(1) TimeRange.isCompatible.simps(2))
+    apply (smt (verit, ccfv_threshold) Semantics.minOpt.elims TimeRange.isCompatible.simps(1) TimeRange.isCompatible.simps(2) TimeRange.isCompatible.simps(4))
+    apply (cases c1)
+    apply simp
+    apply (smt (verit, del_insts) Option.option.sel Semantics.minOpt.elims TimeRange.isCompatible.simps(3) TimeRange.isCompatible.simps(4))
+    apply simp
+    apply (cases b2)
+    using isCompatibleIdempotentToCombineInterval apply force
+    apply (cases c2)
+     apply force
+    by simp
+  done
+
+lemma compatibleIdempotency2 :
+  "isCompatible (x, y) (combineIntervals b c) \<Longrightarrow> isCompatible (x, y) c"
+  apply (cases b)
+  apply (cases c)
+  subgoal for b1 b2 c1 c2
+    apply (simp only:combineIntervals.simps)
+    apply (cases b1)
+    apply (cases c1)
+    apply (smt (verit, ccfv_SIG) Semantics.maxOpt.simps(1) Semantics.minOpt.elims TimeRange.isCompatible.simps(1) TimeRange.isCompatible.simps(2))
+    apply simp
+    apply (smt (verit, best) Semantics.minOpt.elims TimeRange.isCompatible.simps(3) TimeRange.isCompatible.simps(4))
+    apply (cases c1)
+    apply simp
+    apply (smt (verit, best) Option.option.discI Pair_inject Semantics.minOpt.elims TimeRange.isCompatible.elims(1) TimeRange.isCompatible.simps(4))
+    apply simp
+    apply (cases b2)
+    using isCompatibleIdempotentToCombineInterval apply force
+    apply (cases c2)
+     apply force
+    by simp
+  done
+
+lemma compatibleIdempotencyWhen :
+  "b \<le> a2 \<Longrightarrow> b \<le> a1 \<Longrightarrow>
+   isCompatible (a1, a2) (calculateTimeInterval n ct (When a b c)) \<Longrightarrow>
+   isCompatible (a1, a2) (calculateTimeInterval n ct c)"
+  apply (induction a)
+  apply (smt (verit, best) Semantics.calculateTimeInterval.simps(4) TimeRange.isCompatible.simps(2) compatibleIdempotency2)
+  subgoal for c1 c2
+    apply (cases c1)
+    apply simp
+    apply (cases "gtIfNone n 0")
+     apply simp
+    using compatibleIdempotency2 apply blast
+    by presburger
+  done
+
+lemma calculateTimeIntervalAvoidsAmbiguousInterval_When :
+   "isCompatible (x, y) (calculateTimeInterval n ct (When a b c)) \<Longrightarrow>
+    y < b \<or> x \<ge> b"
+  apply (induction a arbitrary:x y n ct b c)
+  subgoal for x y n ct b c
+    apply (cases "ct < b")
+     apply simp
+    apply auto
+    using TimeRange.isCompatible.simps(3) compatibleIdempotency1 by blast
+  subgoal for a1 a2 x y n ct b c
+    apply (cases a1)
+    apply (simp only:calculateTimeInterval.simps)
+    subgoal for a ac
+      apply (cases "gtIfNone n 0")
+       apply simp
+      using compatibleIdempotency2 apply blast
+      by simp
+    done
+  done
+
+lemma calculateTimeIntervalAvoidsAmbiguousInterval_reduceContractStep :
+"isCompatible (timeInterval env) (calculateTimeInterval n ct contract) \<Longrightarrow>
+ reduceContractStep env state contract \<noteq> AmbiguousTimeIntervalReductionError"
+  apply (cases contract)
+  apply (cases "refundOne (accounts state)")
+  apply auto[1]
+       apply auto[1]
+  subgoal for a b c d e
+    by (auto split:bool.splits simp add:Let_def)
+     apply simp
+  subgoal for a b c
+    apply (auto split:prod.splits)
+    subgoal for x y
+      using calculateTimeIntervalAvoidsAmbiguousInterval_When by blast
+    done
+  apply (simp add:Let_def)
+  by simp
+
+lemma resultOfReduceIsCompatibleToo :
+  "isCompatible (timeInterval env) (calculateTimeInterval n ct contract) \<Longrightarrow>
+   reduceContractStep env state contract = Reduced x11 x12 x13 x14 \<Longrightarrow>
+   isCompatible (timeInterval env) (calculateTimeInterval n ct x14)"
+  apply (cases contract)
+  using reduceStepClose_is_Close apply blast
+  subgoal for a b c d e
+    apply (cases "evalValue env state d \<le> 0")
+    by (simp_all add:Let_def)
+     apply (smt (verit, best) Semantics.ReduceStepResult.inject Semantics.calculateTimeInterval.simps(3) Semantics.reduceContractStep.simps(3) TimeRange.isCompatible.elims(2) compatibleIdempotency1 compatibleIdempotency2)
+  subgoal for a b c
+    apply (cases "timeInterval env")
+    apply (simp only:reduceContractStep.simps Let_def prod.case)
+    subgoal for a1 a2
+      apply (cases "a2 < b")
+       apply simp
+      apply simp
+      apply (cases "b \<le> a1")
+       apply simp
+       apply (meson compatibleIdempotencyWhen linorder_not_le)
+      by simp
+    done
+  apply (metis Semantics.ReduceStepResult.inject Semantics.calculateTimeInterval.simps(6) Semantics.reduceContractStep.simps(5))
+  by simp
+
+
+lemma resultOfReductionLoopQuiescentIsCompatibleToo :
+  "isCompatible (timeInterval env) (calculateTimeInterval n ct contract) \<Longrightarrow>
+   reductionLoop b env state contract wa ef = ContractQuiescent x11 x12 x13 x14 x15 \<Longrightarrow>
+   isCompatible (timeInterval env) (calculateTimeInterval n ct x15)"
+  apply (induction b env state contract wa ef rule:reductionLoop.induct)
+  subgoal for reduced env state contract warnings payments
+    apply (simp only:reductionLoop.simps[of reduced env state contract warnings payments])
+    apply (cases "reduceContractStep env state contract")
+    subgoal for warning effect newState ncontract
+      apply (simp only:Let_def ReduceStepResult.case)
+      using resultOfReduceIsCompatibleToo by presburger
+     apply force
+    by simp
+  done
+
+lemma resultOfReduceUntilQuiescentIsCompatibleToo :
+  "isCompatible (timeInterval env) (calculateTimeInterval n ct contract) \<Longrightarrow>
+   reduceContractUntilQuiescent env state contract = ContractQuiescent x11 x12 x13 x14 x15 \<Longrightarrow>
+   isCompatible (timeInterval env) (calculateTimeInterval n ct x15)"
+  by (metis Semantics.reduceContractUntilQuiescent.simps resultOfReductionLoopQuiescentIsCompatibleToo)
+
+lemma calculateTimeIntervalAvoidsAmbiguousInterval_reduceContractUntilQuiescent :
+"isCompatible (timeInterval env) (calculateTimeInterval n ct contract) \<Longrightarrow>
+ reductionLoop b env state contract wa err \<noteq> RRAmbiguousTimeIntervalError"
+  apply (induction b env state contract wa err rule:reductionLoop.induct)
+  subgoal for reduced env state contract warnings payments
+    apply (simp only:reductionLoop.simps[of reduced env state contract warnings payments])
+    apply (cases "reduceContractStep env state contract")
+      apply (simp only:ReduceStepResult.case Let_def)
+    using resultOfReduceIsCompatibleToo apply presburger
+     apply simp
+    using calculateTimeIntervalAvoidsAmbiguousInterval_reduceContractStep by auto
+  done
+
+fun childCase :: "Contract \<Rightarrow> Case list \<Rightarrow> bool" where
+"childCase c Nil = False" |
+"childCase c (Cons (Case _ h) t) = ((h = c) \<or> childCase c t)"
+
+lemma successInApplyCasesReturnChildCase :
+"applyCases env sta h l = Applied nwa nsta ncont \<Longrightarrow> childCase ncont l"
+  apply (induction l)
+   apply simp
+  subgoal for f t
+    apply (cases h)
+      apply (cases f)
+    subgoal for x11 x12 x13 x14 x1 x2
+      apply (cases x1)
+      apply (meson Semantics.ApplyResult.inject)
+        apply (metis Semantics.ApplyResult.inject Semantics.applyCases.simps(1) TimeRange.childCase.simps(2))
+       apply simp
+      by simp
+    apply (cases f)
+    subgoal for x21 x22 x1 x2
+      apply (cases x1)
+        apply simp
+       apply (metis Semantics.ApplyResult.inject Semantics.applyCases.simps(2) TimeRange.childCase.simps(2))
+      by simp
+    apply (cases f)
+    subgoal for x1 x2
+      apply (cases x1)
+    apply simp
+    apply simp
+      by (metis Semantics.ApplyResult.inject Semantics.applyCases.simps(3) TimeRange.childCase.simps(2))
+    done
+  done
+
+lemma resultOfApplyCaseIsCompatibleToo_aux :
+"isCompatible (timeInterval env) (calculateTimeInterval n ct (When x41 x42 x43)) \<Longrightarrow>
+ childCase ncont x41 \<Longrightarrow> ct < x42 \<Longrightarrow> gtIfNone n 0 \<Longrightarrow>
+ isCompatible (timeInterval env) (calculateTimeInterval (subIfSome n 1) ct ncont)"
+  apply (induction x41)
+   apply simp
+  subgoal for h t
+    apply (cases h)
+    subgoal for x y
+      apply simp
+    by (smt (verit, best) TimeRange.isCompatible.elims(3) compatibleIdempotency1 compatibleIdempotency2)
+  done
+  done
+
+lemma resultOfApplyCaseIsCompatibleToo :
+"isCompatible (timeInterval env) (calculateTimeInterval n ct (When x41 x42 x43)) \<Longrightarrow>
+ applyCases env sta h x41 = Applied nwa nsta ncont \<Longrightarrow> ct < x42 \<Longrightarrow> gtIfNone n 0 \<Longrightarrow>
+ isCompatible (timeInterval env) (calculateTimeInterval (subIfSome n 1) ct ncont)"
+  by (simp add: resultOfApplyCaseIsCompatibleToo_aux successInApplyCasesReturnChildCase)
+
+fun ifCaseLt :: "POSIXTime \<Rightarrow> Contract \<Rightarrow> bool" where
+"ifCaseLt ct (When a b c) = (ct < b)" |
+"ifCaseLt _ _ = True"
+
+lemma resultOfApplyInputIsCompatibleToo :
+"isCompatible (timeInterval env) (calculateTimeInterval n ct cont) \<Longrightarrow>
+ applyInput env sta h cont = Applied nwa nsta ncont \<Longrightarrow> ifCaseLt ct cont \<Longrightarrow> gtIfNone n 0 \<Longrightarrow>
+ isCompatible (timeInterval env) (calculateTimeInterval (subIfSome n 1) ct ncont)"
+  apply (cases cont)
+  apply simp_all
+  by (simp add: resultOfApplyCaseIsCompatibleToo)
+
+lemma geIfNone_redListSize :
+  "geIfNone n (int (length (h # t))) \<Longrightarrow> geIfNone (subIfSome n 1) (int (length t))"
+  by (smt (verit, ccfv_threshold) Semantics.geIfNone.elims(1) Semantics.geIfNone.simps(2) Semantics.subIfSome.elims impossible_Cons of_nat_le_iff)
+
+fun isValidInterval :: "POSIXTime \<times> POSIXTime \<Rightarrow> bool" where
+"isValidInterval (a, b) = (a \<le> b)"
+
+lemma reduceStep_ifCaseLtCt_aux : "isCompatible (a, b) (calculateTimeInterval n ct (When x41 x42 x43)) \<Longrightarrow>
+                                   a \<le> b \<Longrightarrow> env = \<lparr>timeInterval = (a, b)\<rparr> \<Longrightarrow> b < x42 \<Longrightarrow> ct < x42"
+  apply (induction x41)
+   apply simp
+   apply (smt (verit, best) TimeRange.isCompatible.simps(3) compatibleIdempotency1)
+  subgoal for h t
+    apply simp
+    apply (cases h)
+    apply simp
+  using compatibleIdempotency2 by presburger
+  done
+
+lemma reduceStep_ifCaseLtCt : "isCompatible (timeInterval env) (calculateTimeInterval n ct (When x41 x42 x43)) \<Longrightarrow> 
+                               reduceContractStep env state (When x41 x42 x43) = NotReduced \<Longrightarrow> isValidInterval (timeInterval env) \<Longrightarrow> ct < x42"
+  apply (cases env)
+  subgoal for timeInterv
+    apply (cases timeInterv)
+    apply simp
+    subgoal for a b
+      apply (cases "b < x42")
+       apply simp
+      using reduceStep_ifCaseLtCt_aux apply blast
+      by (metis Semantics.ReduceStepResult.distinct(5) Semantics.ReduceStepResult.simps(3))
+    done
+  done
+
+
+lemma reduceLoop_ifCaseLtCt : "isCompatible (timeInterval env) (calculateTimeInterval n ct cont) \<Longrightarrow>
+                               reductionLoop b env state cont wa ef = ContractQuiescent x11 x12 x13 x14 x15 \<Longrightarrow> isValidInterval (timeInterval env) \<Longrightarrow> ifCaseLt ct x15"
+  apply (induction b env state cont wa ef rule:reductionLoop.induct)
+  subgoal for reduced env state contract warnings payments
+  apply (cases "x15 = Close")
+  apply simp
+  apply (cases x15)
+  apply simp
+  apply simp
+  apply simp
+    apply (simp only:reductionLoop.simps[of reduced env state contract warnings payments])
+    apply (cases "reduceContractStep env state contract")
+    apply (simp only:ReduceStepResult.case)
+    using resultOfReduceIsCompatibleToo apply presburger
+    apply (simp only:ReduceStepResult.case ifCaseLt.simps)
+       apply (simp add: reduceStep_ifCaseLtCt)
+    apply force
+    using TimeRange.ifCaseLt.simps(5) apply blast
+    using TimeRange.ifCaseLt.simps(6) by blast
+  done
+
+lemma reduceContractUntilQuiescent_ifCaseLtCt : "isCompatible (timeInterval env) (calculateTimeInterval n ct cont) \<Longrightarrow>
+                                                 reduceContractUntilQuiescent env state cont = ContractQuiescent x11 x12 x13 x14 x15 \<Longrightarrow>
+                                                 isValidInterval (timeInterval env) \<Longrightarrow> ifCaseLt ct x15"
+  apply (simp only:reduceContractUntilQuiescent.simps)
+  by (simp add: reduceLoop_ifCaseLtCt)
+
+lemma calculateTimeIntervalAvoidsAmbiguousInterval_applyAllLoop :
+"geIfNone n (int (length inps)) \<Longrightarrow>
+ isCompatible (timeInterval env) (calculateTimeInterval n ct c) \<Longrightarrow>
+ isValidInterval (timeInterval env) \<Longrightarrow> 
+ applyAllLoop b env s c inps wa ef \<noteq>
+ ApplyAllAmbiguousTimeIntervalError"
+  apply (induction b env s c inps wa ef arbitrary: n ct rule:applyAllLoop.induct)
+  subgoal for contractChanged env state contract inputs warnings payments n ct
+    apply (simp only:applyAllLoop.simps[of contractChanged env state contract inputs warnings payments])
+    apply (cases "reduceContractUntilQuiescent env state contract")
+     apply (simp only:ReduceResult.case)
+    apply (cases inputs)
+    apply (simp only:list.cases)
+      apply force
+     apply (simp only:list.cases)
+    subgoal for x11 x12 x13 x14 x15 h t
+      apply (cases "applyInput env x14 h x15")
+       apply (simp only:ApplyResult.case)
+      subgoal fact for nwa nsta ncont
+        subgoal premises fact
+        apply (rule fact(1)[of x11 x12 x13 x14 x15 h t nwa nsta ncont "subIfSome n 1" "ct"])
+            apply auto
+            apply (simp add: fact(7))
+            using fact(2) geIfNone_redListSize apply auto[1]
+            apply (rule resultOfApplyInputIsCompatibleToo[of env n ct x15 x14 h nwa nsta])
+            using fact(3) fact(5) resultOfReduceUntilQuiescentIsCompatibleToo apply blast
+            apply (simp add: fact(7))
+            using fact(3) fact(4) fact(5) reduceContractUntilQuiescent_ifCaseLtCt apply blast
+            using Semantics.gtIfNone.elims(3) fact(2) of_nat_le_iff by fastforce
+          done
+        by (metis Semantics.ApplyAllResult.distinct(5) Semantics.ApplyResult.simps(5))
+      using calculateTimeIntervalAvoidsAmbiguousInterval_reduceContractUntilQuiescent by auto
+    done
+
+lemma calculateTimeIntervalAvoidsAmbiguousInterval_applyAllInputs :
+"geIfNone n (int (length inps)) \<Longrightarrow>
+ isCompatible (minInterv, maxInterv) (calculateTimeInterval n ct c) \<Longrightarrow>
+ isValidInterval (minInterv, maxInterv) \<Longrightarrow> 
+ applyAllInputs \<lparr> timeInterval = (minInterv, maxInterv) \<rparr> s c inps
+    \<noteq> ApplyAllAmbiguousTimeIntervalError"
+  apply (simp only:applyAllInputs.simps)
+  using calculateTimeIntervalAvoidsAmbiguousInterval_applyAllLoop by auto
+
+theorem calculateTimeIntervalAvoidsAmbiguousInterval :
+  "geIfNone n (int (length (inputs tx))) \<Longrightarrow>
+   isCompatible (interval tx) (calculateTimeInterval n ct c) \<Longrightarrow>
+   computeTransaction tx s c \<noteq> TransactionError TEAmbiguousTimeIntervalError"
+  apply (simp only:computeTransaction.simps Let_def)
+  apply (cases tx)
+  subgoal for interv inps
+    apply (cases interv)
+    subgoal for minInterv maxInterv
+      apply (simp add:Let_def del:applyAllInputs.simps)
+      apply (cases "applyAllInputs \<lparr>timeInterval = (max minInterv (minTime s), maxInterv)\<rparr>
+           (s\<lparr>minTime := max minInterv (minTime s)\<rparr>) c inps")
+      apply simp
+      apply simp
+      apply (simp del:applyAllInputs.simps)
+      by (smt (verit) Semantics.applyAllInputs.simps SemanticsTypes.Environment.select_convs(1) TimeRange.isCompatible.elims(2) TimeRange.isCompatible.simps(1) TimeRange.isCompatible.simps(2) TimeRange.isCompatible.simps(3) TimeRange.isCompatible.simps(4) TimeRange.isValidInterval.simps calculateTimeIntervalAvoidsAmbiguousInterval_applyAllLoop)
+    done
+  done
+end
